theories/std/record4.v
@@ -14,9 +14,9 @@ Section heap_GS.
   Definition record4_make : val :=
     λ: "v₀" "v₁" "v₂" "v₃",
       let: "l" := AllocN #4 "v₀" in
-      "l".[1] <- "v₁" ;;
-      "l".[2] <- "v₂" ;;
-      "l".[3] <- "v₃" ;;
+      "l".[#1] <- "v₁" ;;
+      "l".[#2] <- "v₂" ;;
+      "l".[#3] <- "v₃" ;;
       "l".
 
   Definition record4_model l dq₀ v₀ dq₁ v₁ dq₂ v₂ dq₃ v₃ : iProp Σ :=
